<?xml version="1.0"?>


<!DOCTYPE rdf:RDF [
    <!ENTITY owl "http://www.w3.org/2002/07/owl#" >
    <!ENTITY xsd "http://www.w3.org/2001/XMLSchema#" >
    <!ENTITY owl2xml "http://www.w3.org/2006/12/owl2-xml#" >
    <!ENTITY rdfs "http://www.w3.org/2000/01/rdf-schema#" >
    <!ENTITY geol "http://sweet.jpl.nasa.gov/2.0/geol.owl" >
    <!ENTITY chem "http://sweet.jpl.nasa.gov/2.0/chem.owl" >
    <!ENTITY chem2 "http://sweet.jpl.nasa.gov/2.0/chem.owl#" >
    <!ENTITY geol2 "http://sweet.jpl.nasa.gov/2.0/geol.owl#" >
    <!ENTITY basin "http://sweet.jpl.nasa.gov/2.0/geolBasin.owl" >
    <!ENTITY rdf "http://www.w3.org/1999/02/22-rdf-syntax-ns#" >
    <!ENTITY geolBasin "http://sweet.jpl.nasa.gov/2.0/geolBasin.owl#" >
    <!ENTITY planet "http://sweet.jpl.nasa.gov/2.0/astroPlanet.owl" >
    <!ENTITY obj "http://sweet.jpl.nasa.gov/2.0/spaceObject.owl" >
    <!ENTITY spaceObject "http://sweet.jpl.nasa.gov/2.0/spaceObject.owl#" >
    <!ENTITY astroPlanet "http://sweet.jpl.nasa.gov/2.0/astroPlanet.owl#" >
    <!ENTITY petr "http://sweet.jpl.nasa.gov/2.0/geolPetrology.owl" >
    <!ENTITY geolPetrology "http://sweet.jpl.nasa.gov/2.0/geolPetrology.owl#" >
]>


<rdf:RDF xmlns="&basin;#"
     xml:base="http://sweet.jpl.nasa.gov/2.0/geolBasin.owl"
     xmlns:geol2="&geol;#"
     xmlns:basin="http://sweet.jpl.nasa.gov/2.0/geolBasin.owl"
     xmlns:geolPetrology="&petr;#"
     xmlns:spaceObject="&obj;#"
     xmlns:geol="http://sweet.jpl.nasa.gov/2.0/geol.owl"
     xmlns:petr="http://sweet.jpl.nasa.gov/2.0/geolPetrology.owl"
     xmlns:rdfs="http://www.w3.org/2000/01/rdf-schema#"
     xmlns:planet="http://sweet.jpl.nasa.gov/2.0/astroPlanet.owl"
     xmlns:owl2xml="http://www.w3.org/2006/12/owl2-xml#"
     xmlns:chem="http://sweet.jpl.nasa.gov/2.0/chem.owl"
     xmlns:owl="http://www.w3.org/2002/07/owl#"
     xmlns:xsd="http://www.w3.org/2001/XMLSchema#"
     xmlns:rdf="http://www.w3.org/1999/02/22-rdf-syntax-ns#"
     xmlns:obj="http://sweet.jpl.nasa.gov/2.0/spaceObject.owl"
     xmlns:astroPlanet="&planet;#"
     xmlns:geolBasin="&basin;#"
     xmlns:chem2="&chem;#">
    <owl:Ontology rdf:about="">
        <owl:versionInfo>2.0</owl:versionInfo>
        <owl:imports rdf:resource="http://sweet.jpl.nasa.gov/2.0/astroPlanet.owl"/>
        <owl:imports rdf:resource="http://sweet.jpl.nasa.gov/2.0/chem.owl"/>
        <owl:imports rdf:resource="http://sweet.jpl.nasa.gov/2.0/geol.owl"/>
        <owl:imports rdf:resource="http://sweet.jpl.nasa.gov/2.0/geolPetrology.owl"/>
        <owl:imports rdf:resource="http://sweet.jpl.nasa.gov/2.0/spaceObject.owl"/>
    </owl:Ontology>
    


    <!-- 
    ///////////////////////////////////////////////////////////////////////////////////////
    //
    // Object Properties
    //
    ///////////////////////////////////////////////////////////////////////////////////////
     -->

    


    <!-- http://sweet.jpl.nasa.gov/2.0/astroPlanet.owl#hasPlanetaryStructure -->

    <owl:ObjectProperty rdf:about="&planet;#hasPlanetaryStructure"/>
    


    <!-- http://sweet.jpl.nasa.gov/2.0/chem.owl#hasSubstance -->

    <owl:ObjectProperty rdf:about="&chem;#hasSubstance"/>
    


    <!-- http://sweet.jpl.nasa.gov/2.0/geolBasin.owl#hasBasin -->

    <owl:ObjectProperty rdf:about="#hasBasin">
        <rdfs:range rdf:resource="#Basin"/>
    </owl:ObjectProperty>
    


    <!-- 
    ///////////////////////////////////////////////////////////////////////////////////////
    //
    // Classes
    //
    ///////////////////////////////////////////////////////////////////////////////////////
     -->

    


    <!-- http://sweet.jpl.nasa.gov/2.0/geol.owl#GeologicFeature -->

    <owl:Class rdf:about="&geol;#GeologicFeature"/>
    


    <!-- http://sweet.jpl.nasa.gov/2.0/geolBasin.owl#BackArcBasin -->

    <owl:Class rdf:about="#BackArcBasin">
        <rdfs:subClassOf rdf:resource="#Basin"/>
        <rdfs:comment xml:lang="en"
            >Back-arc basins (or retro-arc basins) are geologic features, submarine basins associated with island arcs and subduction zones. They are found at some convergent plate boundaries, presently concentrated in the Western Pacific ocean. [Wikipedia]</rdfs:comment>
    </owl:Class>
    


    <!-- http://sweet.jpl.nasa.gov/2.0/geolBasin.owl#Basin -->

    <owl:Class rdf:about="#Basin">
        <rdfs:subClassOf rdf:resource="&geol;#GeologicFeature"/>
        <rdfs:subClassOf rdf:resource="&obj;#Depression"/>
    </owl:Class>
    


    <!-- http://sweet.jpl.nasa.gov/2.0/geolBasin.owl#FlyschBasin -->

    <owl:Class rdf:about="#FlyschBasin">
        <rdfs:subClassOf rdf:resource="#Basin"/>
        <rdfs:comment xml:lang="en"
            >Flysch is a sequence of sedimentary rocks that is deposited in a deep marine facies in the foreland basin of a developing orogen. Flysch is formed under deep marine circumstances, in a quiet and low-energetic depositional environment. [Wikipedia]</rdfs:comment>
    </owl:Class>
    


    <!-- http://sweet.jpl.nasa.gov/2.0/geolBasin.owl#ForeArcBasin -->

    <owl:Class rdf:about="#ForeArcBasin">
        <rdfs:subClassOf rdf:resource="#Basin"/>
        <rdfs:comment xml:lang="en"
            >A forearc is a depression (basin) in the sea floor located between a subduction zone and an associated volcanic arc. It is typically filled with sediments from the adjacent landmass and the island arc in addition to trapped oceanic crustal material. [Wikipedia]</rdfs:comment>
    </owl:Class>
    


    <!-- http://sweet.jpl.nasa.gov/2.0/geolBasin.owl#ForelandBasin -->

    <owl:Class rdf:about="#ForelandBasin">
        <rdfs:subClassOf rdf:resource="#Basin"/>
        <rdfs:comment xml:lang="en"
            >A foreland basin is a depression that develops adjacent and parallel to a mountain belt. Foreland basins form because the immense mass created by crustal thickening associated with the evolution of a mountain belt causes the lithosphere to bend, by a process known as lithospheric flexure. [Wikipedia]</rdfs:comment>
    </owl:Class>
    


    <!-- http://sweet.jpl.nasa.gov/2.0/geolBasin.owl#IntraArcBasin -->

    <owl:Class rdf:about="#IntraArcBasin">
        <rdfs:subClassOf rdf:resource="#Basin"/>
        <rdfs:comment xml:lang="en"
            >Intra-arc basins are basins that occur between Fore-arc basins and back-arc basins [Wikipedia]</rdfs:comment>
    </owl:Class>
    


    <!-- http://sweet.jpl.nasa.gov/2.0/geolBasin.owl#IntracratonicBasin -->

    <owl:Class rdf:about="#IntracratonicBasin">
        <rdfs:subClassOf rdf:resource="#Basin"/>
        <rdfs:comment xml:lang="en"
            >Intracratonic basins are formed by fluvial sedimentation of an intracratonic area which has undergone sediment sag-loading. [Wikipedia]</rdfs:comment>
    </owl:Class>
    


    <!-- http://sweet.jpl.nasa.gov/2.0/geolBasin.owl#PeripheralForelandBasin -->

    <owl:Class rdf:about="#PeripheralForelandBasin">
        <rdfs:subClassOf rdf:resource="#Basin"/>
        <rdfs:subClassOf>
            <owl:Restriction>
                <owl:onProperty rdf:resource="&planet;#hasPlanetaryStructure"/>
                <owl:allValuesFrom rdf:resource="#FlyschBasin"/>
            </owl:Restriction>
        </rdfs:subClassOf>
        <rdfs:subClassOf>
            <owl:Restriction>
                <owl:onProperty rdf:resource="&chem;#hasSubstance"/>
                <owl:allValuesFrom rdf:resource="&petr;#Molasse"/>
            </owl:Restriction>
        </rdfs:subClassOf>
        <rdfs:comment xml:lang="en"
            >Peripheral (Pro) foreland basins occur on the plate that is subducted or underthrust during plate collision (i.e. the outer arc of the orogen).</rdfs:comment>
    </owl:Class>
    


    <!-- http://sweet.jpl.nasa.gov/2.0/geolBasin.owl#RetroarcForelandBasin -->

    <owl:Class rdf:about="#RetroarcForelandBasin">
        <rdfs:subClassOf rdf:resource="#Basin"/>
        <rdfs:comment xml:lang="en"
            >Retroarc (Retro) foreland basins occur on the plate that overrides during plate convergence or collision (i.e. situated behind the magmatic arc that is linked with the subduction of oceanic lithosphere). [Wikipedia]</rdfs:comment>
    </owl:Class>
    


    <!-- http://sweet.jpl.nasa.gov/2.0/geolBasin.owl#SuccessorBasin -->

    <owl:Class rdf:about="#SuccessorBasin">
        <rdfs:subClassOf rdf:resource="#Basin"/>
        <rdfs:comment xml:lang="en"
            >Successor basins arise from shifting and merging of fore arc, back-arc and intra-arc basins. Basins or sequences that overlap terrane boundaries. [Wikipedia]</rdfs:comment>
    </owl:Class>
    


    <!-- http://sweet.jpl.nasa.gov/2.0/geolBasin.owl#TranspressionalBasin -->

    <owl:Class rdf:about="#TranspressionalBasin">
        <rdfs:subClassOf rdf:resource="#Basin"/>
        <rdfs:comment xml:lang="en"
            >Transpression basins are formed during oblique collision of tectonic plates and during non-orthogonal subduction. [Wikipedia]</rdfs:comment>
    </owl:Class>
    


    <!-- http://sweet.jpl.nasa.gov/2.0/geolBasin.owl#TranstensionalBasin -->

    <owl:Class rdf:about="#TranstensionalBasin">
        <rdfs:subClassOf rdf:resource="#Basin"/>
        <rdfs:comment xml:lang="en"
            >Transtension basins are oblique tensional environments where stretching takes place. [Wikipedia]</rdfs:comment>
    </owl:Class>
    


    <!-- http://sweet.jpl.nasa.gov/2.0/geolPetrology.owl#Molasse -->

    <owl:Class rdf:about="&petr;#Molasse"/>
    


    <!-- http://sweet.jpl.nasa.gov/2.0/spaceObject.owl#Depression -->

    <owl:Class rdf:about="&obj;#Depression"/>
</rdf:RDF>



<!-- Generated by the OWL API (version 2.2.1.1138) http://owlapi.sourceforge.net -->

